equivalence between Ref and Hop1 using equiv directly

compiler/proof_vec/poly1305_corr.ec
@@ -1,4 +1,36 @@
-require import SmtMap Int List FSet.
+require import AllCore SmtMap Int IntDiv List FSet.
+require import Ring.
+import IntID.
+
+(* We have a ring *)
+
+clone import ComRing as Zp.
+
+instance ring with Zp.t
+  op rzero = Zp.zeror
+  op rone  = Zp.oner
+  op add   = Zp.(+)
+  op opp   = Zp.([-])
+  op mul   = Zp.( * )
+  op expr  = Zp.exp
+
+  proof oner_neq0 by apply Zp.oner_neq0 
+  proof addr0     by apply Zp.addr0
+  proof addrA     by apply Zp.addrA
+  proof addrC     by apply Zp.addrC
+  proof addrN     by apply Zp.addrN
+  proof mulr1     by apply Zp.mulr1
+  proof mulrA     by apply Zp.mulrA
+  proof mulrC     by apply Zp.mulrC
+  proof mulrDl    by apply Zp.mulrDl
+  proof expr0     by apply Zp.expr0
+  proof exprS     by apply Zp.exprS.
+
+(* 
+
+
+print ZP.
+
 
 type Zp.
 
@@ -6,6 +38,10 @@ op zero : Zp.
 op one : Zp.
 op ( + ) : Zp -> Zp -> Zp.
 op ( * ) : Zp -> Zp -> Zp.
+op [-] : Zp -> Zp.
+op 
+
+
 
 type Rep.
 
@@ -28,16 +64,16 @@ axiom add_correct x y :
 axiom mul_correct x y :
    safe_mul x y => 
      decode (mul_mod x y) = (decode x) * (decode y).
-
+*)
 (***********************************************)
 (********* Reference implementation ************)
 
-type Zp_msg = (int,Zp) fmap. (* an array *)
+type Zp_msg = (int,Zp.t) fmap. (* an array *)
 
 op ref (m : Zp_msg) (n : int) r =
-  foldl (fun h i => (h + oget m.[i]) * r) zero (iota_ 0 n).
+  foldl (fun h i => (h + oget m.[i]) * r) zeror (iota_ 0 n).
 
-lemma ref0 m r : ref m 0 r = zero.
+lemma ref0 m r : ref m 0 r = zeror.
 proof. by rewrite /ref iota0. qed.
 
 lemma refS m n r : 0 <= n =>
@@ -48,14 +84,13 @@ hint simplify ref0.
 hint simplify refS.
 
 module Poly1305_Ref = {
-   var r : Zp
 
-   proc fold(m : Zp_msg) = {
+   proc fold(r:Zp.t, m : Zp_msg) = {
        var h,n,i;
 
        n <- size (elems (fdom m));
        i <- 0;
-       h <- zero;
+       h <- zeror;
 
        while (i < n) {
          h <- (h + oget m.[i]) * r;
@@ -68,14 +103,13 @@ module Poly1305_Ref = {
 (***********************************************)
 (******************* Unfold ********************)
 module Poly1305_Hop1 = {
-   var r : Zp
 
-   proc fold(m : Zp_msg) = {
+   proc fold(r:Zp.t, m : Zp_msg) = {
        var h,n,i;
 
        n <- size (elems (fdom m));
        i <- 0;
-       h <- zero;
+       h <- zeror;
 
        (* we will go in four parallel tracks,
           4 steps at a time but need at least 
@@ -117,16 +151,15 @@ module Poly1305_Hop1 = {
 (* Parallel tracks *)
 
 module Poly1305_Hop2 = {
-   var r : Zp
 
-   proc fold(m : Zp_msg) = {
+   proc fold(r : Zp.t, m : Zp_msg) = {
        var h,n,i;
        var h1,h2,h3,h4;
        var r2,r3,r4;
 
        n <- size (elems (fdom m));
        i <- 0;
-       h <- zero;
+       h <- zeror;
 
        (* we will go in four parallel tracks,
           4 steps at a time but need at least 
@@ -177,14 +210,14 @@ module Poly1305_Hop2 = {
 }.
 
 (* -------------------------------------------------------------------- *)
-lemma ref_ok m0 :
+lemma ref_ok m0 r0 :
   hoare [ Poly1305_Ref.fold :
-    m = m0 ==> res = ref m0 (size (elems (fdom m0))) Poly1305_Ref.r ].
+    m = m0 /\ r = r0 ==> res = ref m0 (size (elems (fdom m0))) r0 ].
 proof.
 proc; sp.
 conseq (_ :
-      0 <= i /\ i <= n /\ h = ref m i Poly1305_Ref.r
-  ==> h = ref m n Poly1305_Ref.r) => />.
+      0 <= i /\ i <= n /\ h = ref m i r
+  ==> h = ref m n r) => />.
 + by move=> /> &hr; rewrite size_ge0.
 while (#pre); auto => />.
 + by move=> &hr /= ge0i; rewrite refS //#.
@@ -196,20 +229,20 @@ lemma ref_ll : islossless Poly1305_Ref.fold.
 proof. by islossless; while true (n-i) => *; auto => /#. qed.
 
 (* -------------------------------------------------------------------- *)
-lemma ref_ok_ll m0 :
+lemma ref_ok_ll m0 r0 :
   phoare [ Poly1305_Ref.fold :
-    m = m0 ==> res = ref m0 (size (elems (fdom m0))) Poly1305_Ref.r ] = 1%r.
-proof. by conseq ref_ll (ref_ok m0). qed.
+    m = m0 /\ r = r0 ==> res = ref m0 (size (elems (fdom m0))) r0 ] = 1%r.
+proof. by conseq ref_ll (ref_ok m0 r0). qed.
 
 (* -------------------------------------------------------------------- *)
-lemma hop1_ok m0 :
+lemma hop1_ok m0 r0:
   hoare [ Poly1305_Hop1.fold :
-    m = m0 ==> res = ref m0 (size (elems (fdom m0))) Poly1305_Hop1.r ].
+    m = m0 /\ r = r0 ==> res = ref m0 (size (elems (fdom m0))) r0 ].
 proof.
 proc; sp.
 conseq (_ :
-      i = 0 /\ 0 <= i /\ i <= n /\ h = ref m i Poly1305_Hop1.r
-  ==> h = ref m n Poly1305_Hop1.r) => />.
+      i = 0 /\ 0 <= i /\ i <= n /\ h = ref m i r
+  ==> h = ref m n r) => />.
 + by move=> /> &hr; rewrite size_ge0.
 seq 1 : #[2:]pre; [if => //|]; last first.
 + while (#pre); auto => />.
@@ -220,7 +253,7 @@ seq 6 : (#post /\ i <= n - 4); last first.
 seq 5 : #post; first auto => />.
   (* FIXME: hint rewrite should work here *)
 + move=> &hr; rewrite (refS _ 3) // (refS _ 2) //.
-  by rewrite (refS _ 1) // (refS _ 0) // ref0 add0m /#.
+  by rewrite (refS _ 1) // (refS _ 0) // ref0 add0r /#.
 by while (#pre) => //; auto; smt(refS).
 qed.
 
@@ -232,17 +265,94 @@ proof. islossless.
 qed.
 
 (* -------------------------------------------------------------------- *)
-lemma hop1_ok_ll m0 :
+lemma hop1_ok_ll m0 r0 :
   phoare [ Poly1305_Hop1.fold :
-    m = m0 ==> res = ref m0 (size (elems (fdom m0))) Poly1305_Hop1.r ] = 1%r.
-proof. by conseq hop1_ll (hop1_ok m0). qed.
+    m = m0 /\ r = r0 ==> res = ref m0 (size (elems (fdom m0))) r0 ] = 1%r.
+proof. by conseq hop1_ll (hop1_ok m0 r0). qed.
 
 (* -------------------------------------------------------------------- *)
 lemma ref_hop1 :
   equiv [Poly1305_Ref.fold ~ Poly1305_Hop1.fold :
-    ={arg} /\ Poly1305_Ref.r{1} = Poly1305_Hop1.r{2} ==> ={res}
+    ={m,r} ==> ={res}
   ].
-proof.                          (* WTF? *)
-proc*; exists* m{1}, m{2}; elim* => m1 m2.
-by call {1} (ref_ok_ll m1); call {2} (hop1_ok_ll m2); auto.
+proof.                          
+proc*; exists* m{1}, r{1}; elim* => m1 r1.
+call {1} (ref_ok_ll m1 r1); call {2} (hop1_ok_ll m1 r1); auto => />. (* WTF *)
+by move=> &1 &2 !->.
 qed.
+
+(* -------------------------------------------------------------------- *)
+(* Try to prove the equivalence between hop1 and hop2 using equiv       *)
+
+equiv Hop1 : Poly1305_Ref.fold ~ Poly1305_Hop1.fold : 
+                   ={m,r} ==> ={res}.
+proof.
+  proc.
+  seq 3 3 : (={m,r,n,h,i} /\ i{1} = 0 /\ h{1} = Zp.zeror); 1: by auto.
+  if{2}; last by sim.
+  rcondt{1} 1; 1: by move=> &1;auto => /#.
+  rcondt{1} 3; 1: by move=> &1;auto => /#.
+  rcondt{1} 5; 1: by move=> &1;auto => /#.
+  rcondt{1} 7; 1: by move=> &1;auto => /#.
+  seq 8 5 : (={m,r,n,h,i} /\ i{2} = 4 /\ (8 <=  n){2}).
+  + by auto => /> &m2 ?; ring.
+  splitwhile{1} 1 : (8 <= n - i \/ ! (4 %| i)).
+  seq 1 1 : (={m,r,n,h,i} /\ (4 <= n - i < 8){2}).
+  + async while [ (fun r => i%r < r), (i{1}+4)%r ] 
+                [ (fun r => i%r < r), (i{2}+4)%r ] 
+                ( (8 <= n - i \/ ! (4 %| i)){1} /\ (8 <= n - i){2})
+                (!(8 <= n - i){2}) :
+                (={m,r,n,h,i} /\ 4 %| i{2} /\ 4 <= (n - i){2}).
+    + by move=> /> /#.
+    + by move=> /> /#.
+    + by move=> /> /#.        
+    + by move=> &m2;exfalso => &m1 [#] !->> /#.
+    + by move=> &m2;exfalso => &m1 [#] !->> /#.
+    + move=> v1 v2 /=.
+      rcondt{2} 1;1: by auto => /> /#.
+      rcondf{2} 6;1: by auto => /> /#.
+      rcondt{1} 1;1: by auto => /> /#.
+      rcondt{1} 3. 
+      + move=> &m1;auto => /> hd h4 [#] h{h} h8;split; 2: smt().
+        split;[smt() | right].
+        apply /negP => /(dvdzB _ _ _ hd).
+        by rewrite (_: i{m1} - (i{m1} + 1) = -1) //; 1:ring.
+      rcondt{1} 5. 
+      + move=> &m1;auto => /> hd h4 [#] h{h} h8;split; 2: smt().
+        split;[smt() | right].
+        apply /negP => /(dvdzB _ _ _ hd).
+        by rewrite (_: i{m1} - (i{m1} + 1 + 1) = -2) //; 1:ring.
+      rcondt{1} 7. 
+      + move=> &m1;auto => /> hd h4 [#] h{h} h8;split; 2: smt().
+        split;[smt() | right].
+        apply /negP => /(dvdzB _ _ _ hd).
+        by rewrite (_: i{m1} - (i{m1} + 1 + 1 + 1) = -3) //; 1:ring.
+      rcondf{1} 9; 1: by move=> &m1;auto => /> /#.
+      auto => /> &m2 hd hle h{h} h8;split; 1: smt().
+      split; 2: smt().
+      by apply dvdzD.
+    + by islossless; while true (n-i); auto => /#.
+    + by islossless; while true (n-i); auto => /#.
+    by auto => /> /#.
+  rcondt{1} 1; 1: by move=> &1;auto => /#.
+  rcondt{1} 3; 1: by move=> &1;auto => /#.
+  rcondt{1} 5; 1: by move=> &1;auto => /#.
+  rcondt{1} 7; 1: by move=> &1;auto => /#.
+  sim;auto => /> /#.
+qed.
+
+(* -------------------------------------------------------------------- *)
+equiv Hop2 : Poly1305_Hop1.fold ~ Poly1305_Hop2.fold : ={m,r} ==> ={res}.
+proof.
+  proc.
+  while (={h,i,n,m,r}); 1: by sim.
+  seq 3 3 : (={h,i,n,m,r}); 1: by sim.
+  if => //; wp.
+  while (={i,n,m,r} /\ h{1}*r4{2} = (h1*r4 + h2*r3 + h3*r2 + h4*r){2} /\
+         (r4 = exp r 4 /\ r3 = exp r 3 /\ r2 = exp r 2) {2}).
+  + by wp;skip => /> &m1 &m2 heq hle; ring heq.
+  wp;skip => /> &m2 hle;split.
+  + by do !(split;try by ring).
+  by move=> h h1 h2 h3 h4 i _ _ heq _ _ _;ring heq.
+qed.
+
